Rename the indexes of DLList

steel/Learn.Steel.DLList.Data.fst
@@ -12,61 +12,61 @@ module Mem = Steel.Memory
 
 (**** Definition of the vprop *)
 
-let rec dllist_tp (p : list_param) (entry : ref p.r) (len : nat) (exit : ref p.r)
-  : Tot (TP.tprop (dllist_sel_t p entry len exit)) (decreases len)
+let rec dllist_tp (p : list_param) (hd : ref p.r) (len : nat) (lt : ref p.r)
+  : Tot (TP.tprop (dllist_sel_t p hd len lt)) (decreases len)
   = TP.(
     if len = 0
-    then return (dll_nil entry exit)
+    then return (dll_nil hd lt)
     else begin
-      let len' = len - 1 in
-      c   <-- vprt (t_of (vcell p entry)) (vcell p entry); 
-      let c      = (p.cell entry).cl_f c in
-      let entry' = c.cl_nxt              in
-      sl1 <-- tpr (dllist_tp p entry' len' exit);
-      _   <-- tpure (sl1.dll_prv == entry);
-      return #(dllist_sel_t p entry len exit) (dll_cons #p #entry #entry' #len' #exit c sl1)
+      let len' = len - 1            in
+      c   <-- vprt (t_of (vcell p hd)) (vcell p hd); 
+      let c    = (p.cell hd).cl_f c in
+      let hd'  = c.cl_nxt           in
+      sl1 <-- tpr (dllist_tp p hd' len' lt);
+      _   <-- tpure (sl1.dll_prv == hd);
+      return #(dllist_sel_t p hd len lt) (dll_cons #p #hd #hd' #len' #lt c sl1)
     end
   )
 
-let dllist_sl (p : list_param) entry len exit =
-  (dllist_tp p entry len exit).t_hp
+let dllist_sl (p : list_param) hd len lt =
+  (dllist_tp p hd len lt).t_hp
 
-let dllist_sel (p : list_param) entry len exit =
-  (dllist_tp p entry len exit).t_sel
+let dllist_sel (p : list_param) hd len lt =
+  (dllist_tp p hd len lt).t_sel
 
 
 (**** Intro/Elim lemmas *)
 
 let rew () = T.norm [delta_only [`%dllist_tp]; zeta]
 
-let dllist_nil_interp (p : list_param) (entry : ref p.r) (exit : ref p.r) (m : Mem.mem)
+let dllist_nil_interp (p : list_param) (hd : ref p.r) (lt : ref p.r) (m : Mem.mem)
   =
-    let tp = dllist_tp p entry 0 exit in
-    assert (Mem.interp (hp_of (dllist p entry 0 exit)) m /\
-            sel_of (dllist p entry 0 exit) m == dll_nil entry exit)
+    let tp = dllist_tp p hd 0 lt in
+    assert (Mem.interp (hp_of (dllist p hd 0 lt)) m /\
+            sel_of (dllist p hd 0 lt) m == dll_nil hd lt)
       by T.(let _ = TP.pose_interp_lemma (`(`@tp)) (``@m) rew [1] in smt ())
 
-let dllist_cons_interp (p : list_param) (entry : ref p.r) (len : nat) (exit : ref p.r) (m : Mem.mem)
+let dllist_cons_interp (p : list_param) (hd : ref p.r) (len : nat) (lt : ref p.r) (m : Mem.mem)
   =
-    let tp = dllist_tp p entry (len + 1) exit in
-    assert (Mem.interp (hp_of (dllist p entry (len + 1) exit)) m
-         <==> Mem.interp (hp_of (vcell p entry)) m /\
-           (let      c = (p.cell entry).cl_f (sel_of (vcell p entry) m) in
-            let entry' = c.cl_nxt                                       in
-            Mem.interp (hp_of (vcell p entry) `Mem.star` hp_of (dllist p entry' len exit)) m /\
-           (let sl1 : dllist_sel_t p entry' len exit
-                    = sel_of (dllist p entry' len exit) m               in
-            sl1.dll_prv == entry)))
+    let tp = dllist_tp p hd (len + 1) lt in
+    assert (Mem.interp (hp_of (dllist p hd (len + 1) lt)) m
+         <==> Mem.interp (hp_of (vcell p hd)) m /\
+           (let c   = (p.cell hd).cl_f (sel_of (vcell p hd) m) in
+            let hd' = c.cl_nxt                                 in
+            Mem.interp (hp_of (vcell p hd) `Mem.star` hp_of (dllist p hd' len lt)) m /\
+           (let sl1 : dllist_sel_t p hd' len lt
+                    = sel_of (dllist p hd' len lt) m           in
+            sl1.dll_prv == hd)))
       by T.(let _ = TP.pose_interp_lemma (`(`@tp)) (``@m) rew [2] in smt ())
 
 let dllist_cons_sel_eq
-      (p : list_param) (entry : ref p.r) (len : nat) (exit : ref p.r) (m : Mem.mem)
+      (p : list_param) (hd : ref p.r) (len : nat) (lt : ref p.r) (m : Mem.mem)
   =
-    let tp = dllist_tp p entry (len + 1) exit in
-    dllist_cons_interp p entry len exit m;
-    assert (dllist_cons_interp p entry len exit m;
-            let c      = (p.cell entry).cl_f (sel_of (vcell p entry) m) in
-            let entry' = c.cl_nxt                                       in
-            let sl1    = sel_of (dllist p entry' len exit) m            in
-            sel_of (dllist p entry (len + 1) exit) m == dll_cons #p #entry #entry' #len #exit c sl1)
+    let tp = dllist_tp p hd (len + 1) lt in
+    dllist_cons_interp p hd len lt m;
+    assert (dllist_cons_interp p hd len lt m;
+            let c   = (p.cell hd).cl_f (sel_of (vcell p hd) m) in
+            let hd' = c.cl_nxt                                 in
+            let sl1 = sel_of (dllist p hd' len lt) m           in
+            sel_of (dllist p hd (len + 1) lt) m == dll_cons #p #hd #hd' #len #lt c sl1)
       by T.(let _ = TP.pose_interp_lemma (`(`@tp)) (``@m) rew [2] in smt ())
